case_study/RiscvPmp/BlockVer/Verifier.v
@@ -289,10 +289,6 @@ Section BlockVerificationDerived.
       unfold cexec_triple_addr, sexec_triple_addr.
       rsolve.
       iApply rexec_block_addr; rsolve.
-      rewrite !forgetting_trans.
-      iModIntro.
-      iModIntro.
-      rsolve.
     Qed.
 
     Lemma rblock_verification_condition {Σ : LCtx}
@@ -667,10 +663,6 @@ Section AnnotatedBlockVerification.
       unfold cexec_annotated_block_triple_addr, sexec_annotated_block_triple_addr.
       rsolve.
       iApply rexec_annotated_block_addr; rsolve.
-      rewrite !forgetting_trans.
-      iModIntro.
-      iModIntro.
-      rsolve.
     Qed.
 
     Lemma rannotated_block_verification_condition {Σ}
